# Exercise 1.13

Proof that the nth fibonacci number, denoted as $F(n)$, is exactly
$\frac{\phi^n - \psi^n}{\sqrt{5}}$, where $\phi = \frac{1 + \sqrt{5}}{2}$ and
$\psi = \frac{1 - \sqrt{5}}{2}$.

We use an inductive proof. First we show the base cases for the first and second
fibonacci numbers $F(0)$ and $F(1)$.

substituting for $n = 0$ we got

```math
\frac{\phi^0 - \psi^0}{\sqrt{5}} = \frac{1 - 1}{\sqrt{5}} = 0 = F(0)
```

substituting for $n = 1$ we got

```math
\frac{\phi - \psi}{\sqrt{5}} = \frac{1 + \sqrt{5} - 1 + \sqrt{5}}{2\sqrt{5}} = 1 = F(1)
```

Next we proof the inductive case.

Using the squares of $\phi$ and $\psi$

```math
\phi^2 = \frac{1 + \sqrt{5}}{2}^2 = \frac{6 + 2\sqrt{5}}{4} = \frac{3 + \sqrt{5}}{2}\\
\psi^2 = \frac{1 - \sqrt{5}}{2}^2 = \frac{6 - 2\sqrt{5}}{4} = \frac{3 - \sqrt{5}}{2}
```

And assuming that

```math
F(n-1) = \frac{\phi^{n-1} - \psi^{n-1}}{\sqrt{5}}\\
F(n-2) = \frac{\phi^{n-2} - \psi^{n-2}}{\sqrt{5}}
```

By the definition of $F(n) = F(n-1) + F(n-2)$ we complete the proof

```math
\frac{\phi^{n-1} - \psi^{n-1}}{\sqrt{5}} + \frac{\phi^{n-2} - \psi^{n-2}}{\sqrt{5}}\\
= \frac{\phi^{n-2}(\phi + 1) - \psi^{n-2}(\psi + 1)}{\sqrt{5}}\\
= \frac{\phi^{n-2}(\frac{3 + 2\sqrt{5}}{2}) - \psi^{n-2}(\frac{3 - 2\sqrt{5}}{2})}{\sqrt{5}}\\
= \frac{\phi^{n-2}(\phi^2) - \psi^{n-2}(\psi^2)}{\sqrt{5}}\\
= \frac{\phi^n - \psi^n}{\sqrt{5}} = F(n)
```
